refactored

Primitive_Matchers/IpAddresses.thy
@@ -42,24 +42,31 @@ apply(simp add: ipv4range_set_from_netmask_def)
 done
 
 
+
 (*We need a separate ipv4addr syntax thy*)
- (*TODO: Move*)
- fun ipt_ipv4range_to_intervall :: "ipt_ipv4range \<Rightarrow> (ipv4addr \<times> ipv4addr)" where
-    "ipt_ipv4range_to_intervall (Ip4Addr addr) = (ipv4addr_of_dotdecimal addr, ipv4addr_of_dotdecimal addr)" |
-    "ipt_ipv4range_to_intervall (Ip4AddrNetmask pre len) = (
+  fun ipv4cidr_to_intervall :: "(ipv4addr \<times> nat) \<Rightarrow> (ipv4addr \<times> ipv4addr)" where
+    "ipv4cidr_to_intervall (pre, len) = (
       let netmask = (mask len) << (32 - len);
-          network_prefix = (ipv4addr_of_dotdecimal pre AND netmask)
+          network_prefix = (pre AND netmask)
       in (network_prefix, network_prefix OR (NOT netmask))
-     )" 
-
+     )"
+  lemma ipv4cidr_to_intervall: "ipv4cidr_to_intervall (base, len) = (s,e) \<Longrightarrow> ipv4range_set_from_bitmask base len = {s .. e}"
+    apply(simp add: Let_def)
+    apply(subst ipv4range_set_from_bitmask_alt)
+    apply(subst(asm) NOT_mask_len32)
+    by (metis NOT_mask_len32 ipv4range_set_from_bitmask_alt ipv4range_set_from_bitmask_alt1 ipv4range_set_from_netmask_def)
   
-lemma ipt_ipv4range_to_intervall: "ipt_ipv4range_to_intervall ip = (s,e) \<Longrightarrow> {s .. e} = ipv4s_to_set ip"
-  apply(cases ip)
-   apply auto[1]
-  apply(simp add: Let_def)
-  apply(subst ipv4range_set_from_bitmask_alt)
-  apply(subst(asm) NOT_mask_len32)
-  by (metis NOT_mask_len32 ipv4range_set_from_bitmask_alt ipv4range_set_from_bitmask_alt1 ipv4range_set_from_netmask_def)
 
+
+
+
+  fun ipt_ipv4range_to_intervall :: "ipt_ipv4range \<Rightarrow> (ipv4addr \<times> ipv4addr)" where
+    "ipt_ipv4range_to_intervall (Ip4Addr addr) = (ipv4addr_of_dotdecimal addr, ipv4addr_of_dotdecimal addr)" |
+    "ipt_ipv4range_to_intervall (Ip4AddrNetmask pre len) = ipv4cidr_to_intervall ((ipv4addr_of_dotdecimal pre), len)" 
+  
+  lemma ipt_ipv4range_to_intervall: "ipt_ipv4range_to_intervall ip = (s,e) \<Longrightarrow> {s .. e} = ipv4s_to_set ip"
+    apply(cases ip)
+    apply(auto simp add: ipv4cidr_to_intervall)
+    done
 
 end
